steel/Veritas.Steel.Verifier.fst
@@ -30,6 +30,13 @@ let check_overflow_add (x y:U64.t)
    else if res -^ x = y then Some res
    else None
 
+val update_clock (ts:T.timestamp) (vs:thread_state_t)
+  : Steel unit
+    (thread_state_inv vs)
+    (fun _ -> thread_state_inv vs)
+    (requires fun _ -> True)
+    (ensures fun h0 _ h1 -> v_thread vs h1 == model_update_clock (v_thread vs h0) ts)
+
 let update_clock (ts:T.timestamp) (vs:thread_state_t) =
   let c = Steel.Reference.read vs.clock in
   let res = check_overflow_add c ts in
@@ -39,23 +46,18 @@ let update_clock (ts:T.timestamp) (vs:thread_state_t) =
   | Some res ->
     write vs.clock res; ()
 
-//Needs an unfold, else weirdness
-unfold
-let slot_ok (s:U16.t) (vs:_) (h:rmem (thread_state_inv vs))
-  = U16.v s < length (v_thread vs h).model_store
-
-val points_to_some_slot (s:U16.t)
+val points_to_some_slot (vs:_)
+                        (s:slot vs.len)
                         (d:bool)
-                        (vs:_)
+
   : Steel bool
     (thread_state_inv vs)
     (fun _ -> thread_state_inv vs)
-    (requires fun h -> U16.v s < length (v_thread vs h).model_store)
+    (requires fun h -> True)
     (ensures fun h0 b h1 ->
-      U16.v s < length (v_thread vs h0).model_store /\
       b == VerifierModel.points_to_some_slot (v_thread vs h0) s d /\
       v_thread vs h0 == v_thread vs h1)
-let points_to_some_slot s d vs
+let points_to_some_slot vs s d
   = let r = vcache_get_record vs.st s in
     match r with
     | None -> false
@@ -64,26 +66,25 @@ let points_to_some_slot s d vs
       then Some? (r.record_l_child_in_store)
       else Some? (r.record_r_child_in_store)
 
-val madd_to_store (s:U16.t) (k:T.key) (v:T.value) (s':U16.t) (d:bool)
-                  (vs:_)
+val madd_to_store (vs:_)
+                  (s:slot vs.len)
+                  (k:T.key)
+                  (v:T.value)
+                  (s':slot vs.len)
+                  (d:bool)
   : Steel unit
     (thread_state_inv vs)
     (fun _ -> thread_state_inv vs)
     (requires fun h0 ->
-      U16.v s < length (v_thread vs h0).model_store /\
-      U16.v s' < length (v_thread vs h0).model_store /\
       not (has_slot (v_thread vs h0) s) /\
       is_value_of k v /\
       has_slot (v_thread vs h0) s')
     (ensures fun h0 _ h1 ->
-      U16.v s < length (v_thread vs h0).model_store /\
-      U16.v s' < length (v_thread vs h0).model_store /\
       v_thread vs h1 == model_madd_to_store (v_thread vs h0) s k v s' d)
 
 #push-options "--query_stats --fuel 0 --ifuel 1"
-let madd_to_store s k v s' d vs
+let madd_to_store vs s k v s' d
   = let h = get () in
-    assert (U16.v s  < length (v_thread vs h).model_store);  //this assert seems necessary
     assert (not (has_slot (v_thread vs h) s)); //this one does too
     let r' = vcache_get_record vs.st s' in
     match r' with
@@ -104,38 +105,28 @@ let madd_to_store s k v s' d vs
       in
       vcache_update_record vs.st s' r'
 
-val madd_to_store_split (s:U16.t) (k:T.key) (v:T.value) (s':U16.t) (d d2:bool)
-                        (vs:_)
+let coerce #a #p (x:a) (pf:squash (p x)) : x:a{p x} = x
+
+val madd_to_store_split (vs:_)
+                        (s:slot vs.len)
+                        (k:T.key)
+                        (v:T.value)
+                        (s':slot vs.len)
+                        (d d2:bool)
+
   : Steel unit
     (thread_state_inv vs)
     (fun _ -> thread_state_inv vs)
     (requires fun h0 ->
-      U16.v s < length (v_thread vs h0).model_store /\
-      U16.v s' < length (v_thread vs h0).model_store /\
       not (has_slot (v_thread vs h0) s) /\
       is_value_of k v /\
       has_slot (v_thread vs h0) s')
     (ensures fun h0 _ h1 ->
-      U16.v s < length (v_thread vs h0).model_store /\
-      U16.v s' < length (v_thread vs h0).model_store /\
       v_thread vs h1 == model_madd_to_store_split (v_thread vs h0) s k v s' d d2)
-let choose d l r = if d then l else r
-let coerce #a #p (x:a) (pf:squash (p x)) : x:a{p x} = x
 
-assume
-val vcache_bounds_check (vst:vstore) (s:slot_id)
-  : Steel bool
-          (is_vstore vst)
-          (fun _ -> is_vstore vst)
-          (requires fun h -> True)
-          (ensures fun h0 res h1 ->
-             res  == (U16.v s < length (asel vst h0)) /\
-             asel vst h0 == asel vst h1)
-
-#push-options "--query_stats --fuel 0 --ifuel 1"
-let madd_to_store_split s k v s' d d2 vs
+#push-options "--fuel 0 --ifuel 1"
+let madd_to_store_split vs s k v s' d d2
   = let h = get () in
-    assert (U16.v s  < length (v_thread vs h).model_store);  //this assert seems necessary
     assert (is_value_of k v);
     assert (not (has_slot (v_thread vs h) s)); //this one does too
     assert (has_slot (v_thread vs h) s');
@@ -147,45 +138,38 @@ let madd_to_store_split s k v s' d d2 vs
       match s2_opt with
       | None -> noop(); ()
       | Some s2 ->
-        let b = vcache_bounds_check vs.st s2 in
-        if not b then (noop(); ())
-        else (
-          let r2 = vcache_get_record vs.st s2 in
-          match r2 with
-          | None -> noop() ; ()
-          | Some r2 ->
-            let pf : squash (is_value_of k v) = () in
-            let v : (v:T.value { is_value_of k v }) =
+        let r2 = vcache_get_record vs.st s2 in
+        match r2 with
+        | None -> noop() ; ()
+        | Some r2 ->
+          let pf : squash (is_value_of k v) = () in
+          let v : (v:T.value { is_value_of k v }) =
               coerce v pf
-            in
-            let e = mk_record_full k v T.MAdd None None (Some p) in
-            let e = record_update_child e d2 s2 in
-            let e' = record_update_child r' d s in
-            let p2new = s2, d2 in
-            let e2 = record_update_parent_slot r2 p2new in
-            vcache_update_record vs.st s e;
-            vcache_update_record vs.st s' e';
-            vcache_update_record vs.st s2 e2
-          )
+          in
+          let e = mk_record_full k v T.MAdd None None (Some p) in
+          let e = record_update_child e d2 s2 in
+          let e' = record_update_child r' d s in
+          let p2new = s2, d2 in
+          let e2 = record_update_parent_slot r2 p2new in
+          vcache_update_record vs.st s e;
+          vcache_update_record vs.st s' e';
+          vcache_update_record vs.st s2 e2
 
 val vevictb_update_hash_clock
-       (s:U16.t)
-       (t:T.timestamp)
        (vs:_)
+       (s:slot vs.len)
+       (t:T.timestamp)
    : Steel unit
      (thread_state_inv vs)
      (fun _ -> thread_state_inv vs)
      (requires fun h0 ->
-       U16.v s < length (v_thread vs h0).model_store /\
        VerifierModel.sat_evictb_checks (v_thread vs h0) s t)
      (ensures fun h0 _ h1 ->
-       U16.v s < length (v_thread vs h0).model_store /\
        VerifierModel.sat_evictb_checks (v_thread vs h0) s t /\
        v_thread vs h1 ==
        model_vevictb_update_hash_clock (v_thread vs h0) s t)
-let vevictb_update_hash_clock s t vs
+let vevictb_update_hash_clock vs s t
   = let h = get () in
-    assert (U16.v s  < length (v_thread vs h).model_store);  //these asserts are necessary
     assert (VerifierModel.sat_evictb_checks (v_thread vs h) s t);
     let r = vcache_get_record vs.st s in
     let Some r = r in
@@ -194,28 +178,24 @@ let vevictb_update_hash_clock s t vs
     PRF.prf_update_hash vs.hevict record t vs.id;
     Steel.Reference.write vs.clock t
 
-let bevict_from_store (s:U16.t) (vs:_)
+let bevict_from_store (vs:_) (s:slot vs.len)
   : Steel unit
     (thread_state_inv vs)
     (fun _ -> thread_state_inv vs)
-    (requires fun h0 ->
-       U16.v s < length (v_thread vs h0).model_store)
+    (requires fun h0 -> True)
     (ensures fun h0 _ h1 ->
-       U16.v s < length (v_thread vs h0).model_store /\
        v_thread vs h1 ==
        model_bevict_from_store (v_thread vs h0) s)
   = vcache_evict_record vs.st s; ()
 
-let update_value (s:U16.t) (v:T.value) (vs:_)
+let update_value (vs:_) (s:slot vs.len) (v:T.value)
   : Steel unit
     (thread_state_inv vs)
     (fun _ -> thread_state_inv vs)
     (requires fun h0 ->
-      U16.v s  < length (v_thread vs h0).model_store /\
       has_slot (v_thread vs h0) s /\
       is_value_of (key_of_slot (v_thread vs h0) s) v)
     (ensures fun h0 _ h1 ->
-      U16.v s  < length (v_thread vs h0).model_store /\
       has_slot (v_thread vs h0) s /\
       is_value_of (key_of_slot (v_thread vs h0) s) v /\
       v_thread vs h1 == model_update_value (v_thread vs h0) s v)
@@ -224,20 +204,15 @@ let update_value (s:U16.t) (v:T.value) (vs:_)
     let r' = { r with record_value = v } in
     vcache_update_record vs.st s r'
 
-let mevict_from_store (s s':_) (d:_) (vs:_)
+let mevict_from_store (vs:_) (s s':slot vs.len) (d:_)
   : Steel unit
     (thread_state_inv vs)
     (fun _ -> thread_state_inv vs)
-    (requires fun h0 ->
-       U16.v s < length (v_thread vs h0).model_store /\
-       U16.v s' < length (v_thread vs h0).model_store)
+    (requires fun h0 -> True)
     (ensures fun h0 _ h1 ->
-       U16.v s < length (v_thread vs h0).model_store /\
-       U16.v s' < length (v_thread vs h0).model_store /\
        v_thread vs h1 ==
        model_mevict_from_store (v_thread vs h0) s s' d)
   = let h = get () in
-    assert (U16.v s  < length (v_thread vs h).model_store);  //this assert seems necessary
     let r' = vcache_get_record vs.st s' in
     match r' with
     | None ->
@@ -256,12 +231,15 @@ let mevict_from_store (s s':_) (d:_) (vs:_)
         vcache_evict_record vs.st s;
         Steel.Effect.Atomic.return ()
 
+let fail (vs:thread_state_t) (msg:string)
+  : SteelF unit
+             (thread_state_inv vs)
+             (fun _ -> thread_state_inv vs)
+             (requires fun _ -> True)
+             (ensures fun h0 _ h1 -> v_thread vs h1 == model_fail (v_thread vs h0))
+  = write vs.failed true; ()
 
-
-#push-options "--query_stats --fuel 0 --ifuel 1"
-let fail vs msg = write vs.failed true; ()
-
-let vget (s:U16.t) (k:T.key) (v:T.data_value) (vs: thread_state_t)
+let vget (vs: thread_state_t) (s:slot vs.len) (k:T.key) (v:T.data_value)
   = let ro = VCache.vcache_get_record vs.st s in
     match ro with
     | None ->
@@ -275,7 +253,7 @@ let vget (s:U16.t) (k:T.key) (v:T.data_value) (vs: thread_state_t)
       else (noop (); ())
 
 (* verifier write operation *)
-let vput s k v vs
+let vput vs s k v
   = let ro = VCache.vcache_get_record vs.st s in
     match ro with
     | None ->
@@ -289,10 +267,9 @@ let vput s k v vs
         () //seem to need this
       )
 
-
-let vaddm s r s' vs
+let vaddm vs s r s'
   = let h = get () in
-    assert (U16.v s  < length (v_thread vs h).model_store);  //this assert seems necessary
+    assert (v_thread vs h == v_thread vs h); //necessary
     let k = r.T.record_key in
     let v = r.T.record_value in
     (* check store contains slot s' *)
@@ -317,33 +294,36 @@ let vaddm s r s' vs
              | T.Dh_vnone _ -> (* k' has no child in direction d *)
              (* first add must be init value *)
                if v <> init_value k then fail vs "incorrect initial value"
-               else let b = points_to_some_slot s' d vs in
-                    if b then fail vs "points to some slot"
-                    else (
-                      let tsm = madd_to_store s k v s' d vs in
-                      let v'_upd = update_merkle_value v' d k h false in
-                      update_value s' (T.V_mval v'_upd) vs
-                    )
+               else (
+                 let b = points_to_some_slot vs s' d in
+                 if b then fail vs "points to some slot"
+                 else (
+                   let tsm = madd_to_store vs s k v s' d in
+                   let v'_upd = update_merkle_value v' d k h false in
+                   let s' : slot vs.len = s' in
+                   update_value vs s' (T.V_mval v'_upd)
+                 )
+               )
 
-        | T.Dh_vsome {T.dhd_key=k2; T.dhd_h=h2; T.evicted_to_blum = b2} ->
-          if k2 = k then (* k is a child of k' *)
-            (* check hashes match and k was not evicted to blum *)
-            if not (h2 = h && b2 = T.Vfalse) then fail vs "hash mismatch or evicted"
-            (* check slot s' does not contain a desc along direction d *)
-            else (
-              let b = points_to_some_slot s' d vs in
-              if b then fail vs "points to some slot"
-              else madd_to_store s k v s' d vs
-            )
-          else (
-            (* first add must be init value *)
-            if v <> init_value k then fail vs "not init value"
-            (* check k2 is a proper desc of k *)
-            else
-              let b = (is_proper_descendent k2 k) in
-                if not b
-                then fail vs "not proper descendent"
-                else (
+             | T.Dh_vsome {T.dhd_key=k2; T.dhd_h=h2; T.evicted_to_blum = b2} ->
+               if k2 = k then (* k is a child of k' *)
+               (* check hashes match and k was not evicted to blum *)
+               if not (h2 = h && b2 = T.Vfalse) then fail vs "hash mismatch or evicted"
+               (* check slot s' does not contain a desc along direction d *)
+               else (
+                 let b = points_to_some_slot vs s' d in
+                 if b then fail vs "points to some slot"
+                 else madd_to_store vs s k v s' d
+               )
+               else (
+               (* first add must be init value *)
+               if v <> init_value k then fail vs "not init value"
+               (* check k2 is a proper desc of k *)
+               else
+                 let b = (is_proper_descendent k2 k) in
+                 if not b
+                 then fail vs "not proper descendent"
+                 else (
                   let pf : squash (is_proper_descendent k2 k) = () in
                   //need this weird coercion to avoid mysterious failures
                   let k : (k:T.key { is_proper_descendent k2 k }) = coerce k pf in
@@ -351,22 +331,22 @@ let vaddm s r s' vs
                   let Some mv = to_merkle_value v in
                   let mv_upd = update_merkle_value mv d2 k2 h2 (b2=T.Vtrue) in
                   let v'_upd = update_merkle_value v' d k h false in
-                  let b = points_to_some_slot s' d vs in
+                  let b = points_to_some_slot vs s' d in
                   //can't share the continuation
                   if b
                   then (
-                    madd_to_store_split s k (T.V_mval mv_upd) s' d d2 vs;
-                    update_value s' (T.V_mval v'_upd) vs
+                    madd_to_store_split vs s k (T.V_mval mv_upd) s' d d2;
+                    update_value vs s' (T.V_mval v'_upd)
                   )
                   else (
-                    madd_to_store s k (T.V_mval mv_upd) s' d vs;
-                    update_value s' (T.V_mval v'_upd) vs
+                    madd_to_store vs s k (T.V_mval mv_upd) s' d;
+                    update_value vs s' (T.V_mval v'_upd)
                   )
              )))
 
-let vevictm s s' vs
+let vevictm vs s s'
   = let h = get () in
-    assert (U16.v s  < length (v_thread vs h).model_store);  //this assert seems necessary
+    assert (v_thread vs h == v_thread vs h);  //this assert seems necessary
     if s = s' then fail vs "Equal slots"
     else (
       let r = VCache.vcache_get_record vs.st s in
@@ -383,8 +363,8 @@ let vevictm s s' vs
         if not (is_proper_descendent k k') then fail vs "Not proper descendent"
         (* check k does not have a (merkle) child in the store *)
         else
-          let b1 = points_to_some_slot s true vs in
-          let b2 = points_to_some_slot s false vs in
+          let b1 = points_to_some_slot vs s true in
+          let b2 = points_to_some_slot vs s false in
           if b1 || b2
           then fail vs "Points to some slot"
           else (
@@ -397,13 +377,13 @@ let vevictm s s' vs
               if k2 <> k then fail vs "k2 <> k"
               else match r.record_parent_slot with
                    | None ->
-                     let b = points_to_some_slot s' d vs in
+                     let b = points_to_some_slot vs s' d in
                      if b then fail vs "parent slot mismatch"
                      else (
                        let h = hashfn v in //TODO: Lower
                        let v'_upd = update_merkle_value v' d k h false in
-                       let tsm = update_value s' (T.V_mval v'_upd) vs in
-                       mevict_from_store s s' d vs
+                       let tsm = update_value vs s' (T.V_mval v'_upd) in
+                       mevict_from_store vs s s' d
                      )
 
                    | Some (p_s, p_d) ->
@@ -412,15 +392,14 @@ let vevictm s s' vs
                      else (
                        let h = hashfn v in //TODO: Lower
                        let v'_upd = update_merkle_value v' d k h false in
-                       let tsm = update_value s' (T.V_mval v'_upd) vs in
-                       mevict_from_store s s' d vs
+                       let tsm = update_value vs s' (T.V_mval v'_upd) in
+                       mevict_from_store vs s s' d
                      )
           ))
 
-let vaddb s r t thread_id vs
+let vaddb vs s r t thread_id
   = let h = get() in
-    assert (U16.v s < length (v_thread vs h).model_store);
-
+    assert (v_thread vs h == v_thread vs h);
     let { T.record_key = k;
           T.record_value = v } = r in
     (* check value type consistent with key k *)
@@ -440,18 +419,17 @@ let vaddb s r t thread_id vs
         VCache.vcache_add_record vs.st s k v T.BAdd)
     )
 
-val sat_evictb_checks (s:U16.t)
+val sat_evictb_checks (vs:_)
+                      (s:slot vs.len)
                       (t:T.timestamp)
-                      (vs:_)
   : Steel bool
     (thread_state_inv vs)
     (fun _ -> thread_state_inv vs)
-    (requires fun h -> U16.v s < length (v_thread vs h).model_store)
+    (requires fun h -> True)
     (ensures fun h0 b h1 ->
-      U16.v s < length (v_thread vs h0).model_store /\
       b == VerifierModel.sat_evictb_checks (v_thread vs h0) s t /\
       v_thread vs h0 == v_thread vs h1)
-let sat_evictb_checks s t vs
+let sat_evictb_checks vs s t
   = let ro = VCache.vcache_get_record vs.st s in
     match ro with
     | None -> Steel.Effect.Atomic.return false
@@ -462,42 +440,30 @@ let sat_evictb_checks s t vs
       else if not (clk `timestamp_lt` t)
       then Steel.Effect.Atomic.return false
       else (
-        let b1 = points_to_some_slot s true vs in
-        let b2 = points_to_some_slot s false vs in
+        let b1 = points_to_some_slot vs s true in
+        let b2 = points_to_some_slot vs s false in
         not b1 && not b2
       )
 
-let vevictb (s:U16.t)
-            (t:T.timestamp)
-            (vs:thread_state_t)
-  : Steel unit
-    (thread_state_inv vs)
-    (fun _ -> thread_state_inv vs)
-    (requires fun h -> U16.v s < length (v_thread vs h).model_store)
-    (ensures  fun h0 _ h1 ->
-      U16.v s < length (v_thread vs h0).model_store /\
-      v_thread vs h1 == vevictb_model (v_thread vs h0) s t)
-  = let chk = sat_evictb_checks s t vs in
+let vevictb vs s t
+  = let chk = sat_evictb_checks vs s t in
     if not chk then fail vs "sat_evictb_checks failed"
     else (
       let Some r = VCache.vcache_get_record vs.st s in
       if r.record_add_method <> T.BAdd
       then fail vs "Record is not a BAdd"
       else (
-        vevictb_update_hash_clock s t vs;
-        bevict_from_store s vs
+        vevictb_update_hash_clock vs s t;
+        bevict_from_store vs s
       )
     )
 
-let vevictbm (s s':U16.t)
-             (t:T.timestamp)
-             (vs:_)
+let vevictbm vs s s' t
   = let h = get() in
-    assert (U16.v s < length (v_thread vs h).model_store);
-    assert (U16.v s' < length (v_thread vs h).model_store);
+    assert (v_thread vs h == v_thread vs h);
     if s = s' then fail vs "equal slots"
     else (
-      let b = sat_evictb_checks s t vs in
+      let b = sat_evictb_checks vs s t in
       if not b then fail vs "sat_evictb_checks"
       else (
         let r' = VCache.vcache_get_record vs.st s' in
@@ -530,10 +496,10 @@ let vevictbm (s s':U16.t)
                        if ps <> s' || pd <> d
                        then fail vs "paren slot checks"
                        else (
-                         vevictb_update_hash_clock s t vs;
+                         vevictb_update_hash_clock vs s t;
                          let mv'_upd = update_merkle_value mv' d k h2 true in
-                         update_value s' (T.V_mval mv'_upd) vs;
-                         mevict_from_store s s' d vs
+                         update_value vs s' (T.V_mval mv'_upd);
+                         mevict_from_store vs s s' d
                        )
                 )
             )
