steel/Veritas.Steel.Verifier.fsti
@@ -22,7 +22,8 @@ let counter_t = ref U64.t
 noeq
 type thread_state_t = {
   id           : T.thread_id;
-  st           : vstore;  //a map from keys (cache ids) to merkle leaf or internal nodes
+  len          : U16.t;
+  st           : vstore len;  //a map from keys (cache ids) to merkle leaf or internal nodes
   clock        : counter_t;
   hadd         : PRF.prf_set_hash; //current incremental set hash values; TODO
   hevict       : PRF.prf_set_hash;
@@ -45,6 +46,7 @@ let v_thread (#p:vprop) (t:thread_state_t)
   : GTot thread_state_model
   = {
       model_thread_id = t.id;
+      model_store_len = t.len;
       model_failed = sel t.failed (focus_rmem h (thread_state_inv t));
       model_store = asel t.st (focus_rmem h (thread_state_inv t));
       model_clock = sel t.clock (focus_rmem h (thread_state_inv t));
@@ -52,99 +54,68 @@ let v_thread (#p:vprop) (t:thread_state_t)
       model_hevict = PRF.v_hash t.hevict (focus_rmem h (thread_state_inv t))
     }
 
-// AF: Requires some integers reasoningm, but should be straightforward
-val update_clock (ts:T.timestamp) (vs:thread_state_t)
-  : Steel unit
-    (thread_state_inv vs)
-    (fun _ -> thread_state_inv vs)
-    (requires fun _ -> True)
-    (ensures fun h0 _ h1 -> v_thread vs h1 == model_update_clock (v_thread vs h0) ts)
-
-val fail (vs:thread_state_t) (msg:string)
-  : SteelF unit
-             (thread_state_inv vs)
-             (fun _ -> thread_state_inv vs)
-             (requires fun _ -> True)
-             (ensures fun h0 _ h1 -> v_thread vs h1 == model_fail (v_thread vs h0))
-
-
-val vget (s:U16.t) (k:T.key) (v:T.data_value) (vs: thread_state_t)
+val vget (vs: thread_state_t) (s:slot vs.len) (k:T.key) (v:T.data_value)
   : Steel unit
           (thread_state_inv vs)
           (fun _ -> thread_state_inv vs)
-          (requires fun h -> U16.v s < length (v_thread vs h).model_store)
+          (requires fun h -> True)
           (ensures fun h0 _ h1 ->
-            U16.v s < length (v_thread vs h0).model_store /\
             v_thread vs h1 == vget_model (v_thread vs h0) s k v
           )
 
-val vput (s:U16.t) (k:T.key) (v:T.data_value) (vs: thread_state_t)
+val vput (vs: thread_state_t) (s:slot vs.len) (k:T.key) (v:T.data_value)
   : Steel unit
     (thread_state_inv vs)
     (fun _ -> thread_state_inv vs)
-    (requires fun h -> U16.v s < length (v_thread vs h).model_store)
+    (requires fun h -> True)
     (ensures fun h0 _ h1 ->
-      U16.v s < length (v_thread vs h0).model_store /\
       v_thread vs h1 == vput_model (v_thread vs h0) s k v)
 
-val vaddm (s:U16.t) (r:T.record) (s':U16.t) (vs:_)
+val vaddm (vs:_) (s:slot vs.len) (r:T.record) (s':slot vs.len)
   : Steel unit
     (thread_state_inv vs)
     (fun _ -> thread_state_inv vs)
-    (requires fun h0 ->
-      U16.v s  < length (v_thread vs h0).model_store /\
-      U16.v s' < length (v_thread vs h0).model_store)
+    (requires fun h0 -> True)
     (ensures fun h0 _ h1 ->
-      U16.v s  < length (v_thread vs h0).model_store /\
-      U16.v s' < length (v_thread vs h0).model_store /\
       v_thread vs h1 == vaddm_model (v_thread vs h0) s r s')
 
-val vevictm (s s':U16.t) (vs:_)
+val vevictm (vs:_) (s s':slot vs.len)
   : Steel unit
     (thread_state_inv vs)
     (fun _ -> thread_state_inv vs)
-    (requires fun h0 ->
-      U16.v s  < length (v_thread vs h0).model_store /\
-      U16.v s' < length (v_thread vs h0).model_store)
+    (requires fun h0 -> True)
     (ensures fun h0 _ h1 ->
-      U16.v s  < length (v_thread vs h0).model_store /\
-      U16.v s' < length (v_thread vs h0).model_store /\
       v_thread vs h1 == vevictm_model (v_thread vs h0) s s')
 
-val vaddb (s:U16.t)
+val vaddb (vs:thread_state_t)
+          (s:slot vs.len)
           (r:T.record)
           (t:T.timestamp)
           (thread_id:T.thread_id)
-          (vs:thread_state_t)
   : Steel unit
     (thread_state_inv vs)
     (fun _ -> thread_state_inv vs)
-    (requires fun h -> U16.v s < length (v_thread vs h).model_store)
+    (requires fun h -> True)
     (ensures fun h0 _ h1 ->
-      U16.v s < length (v_thread vs h0).model_store /\
       v_thread vs h1 == vaddb_model (v_thread vs h0) s r t thread_id)
 
-val vevictb (s:U16.t)
+val vevictb (vs:thread_state_t)
+            (s:slot vs.len)
             (t:T.timestamp)
-            (vs:thread_state_t)
+
   : Steel unit
     (thread_state_inv vs)
     (fun _ -> thread_state_inv vs)
-    (requires fun h -> U16.v s < length (v_thread vs h).model_store)
+    (requires fun h -> True)
     (ensures  fun h0 _ h1 ->
-      U16.v s < length (v_thread vs h0).model_store /\
       v_thread vs h1 == vevictb_model (v_thread vs h0) s t)
 
-val vevictbm (s s':U16.t)
+val vevictbm (vs:_)
+             (s s':slot vs.len)
              (t:T.timestamp)
-             (vs:_)
   : Steel unit
     (thread_state_inv vs)
     (fun _ -> thread_state_inv vs)
-    (fun h0 ->
-      U16.v s < length (v_thread vs h0).model_store /\
-      U16.v s' < length (v_thread vs h0).model_store)
+    (fun h0 -> True)
     (fun h0 _ h1 ->
-      U16.v s < length (v_thread vs h0).model_store /\
-      U16.v s' < length (v_thread vs h0).model_store /\
       v_thread vs h1 == vevictbm_model (v_thread vs h0) s s' t)
